Sparate disk and block_mem in semantics

src/PermHoare.v
@@ -1,4 +1,4 @@
-Require Import Mem.
+Require Import Mem Pred.
 Require Import PermProg PermSec.
 Require Import List.
 Require Import Morphisms.
@@ -11,29 +11,31 @@ Set Implicit Arguments.
 
 Definition pair_args_helper (A B C:Type) (f: A->B->C) (x: A*B) := f (fst x) (snd x).
 
-Definition donecond (T: Type) := state -> T -> Prop.
+Definition donecond (T: Type) := tagged_disk -> block_mem -> T -> Prop.
 
-Definition corr2 (T: Type) pr (pre: perm -> donecond T -> state -> Prop) (p: prog T) :=
-  forall s s' tr tr' done out,
-    pre pr done s
-  -> exec pr s tr p s' out tr'
-  -> (exists v, out = Finished v /\ done s' v).
+Definition corr2 (T: Type) pr (pre: donecond T -> block_mem -> @pred _ _ tagged_block) (p: prog T) :=
+  forall d bm tr tr' donec out,
+    pre donec bm d
+  -> exec pr tr d bm p out tr'
+  -> (exists d' bm' v, out = Finished d' bm' v /\
+                 donec d' bm' v /\
+                 permission_secure d bm pr p).
 
-Notation "{{ pr pre }} p" := (corr2 pr pre p)
+Notation "x= pr : pre =x p" := (corr2 pr pre p)
   (at level 0, p at level 60).
 
 Notation "'RET' : r post" :=
-  (fun s =>
-     (fun r => post s)
-  )
+  (fun F =>
+    (fun r => (F * post)%pred)
+  )%pred
   (at level 0, post at level 90, r at level 0, only parsing).
 
 Notation "'RET' : ^( ra , .. , rb ) post" :=
-  (fun s =>
+  (fun F =>
     (pair_args_helper (fun ra => ..
-      (pair_args_helper (fun rb (_:unit) => post s))
+      (pair_args_helper (fun rb (_:unit) => (F * post)%pred))
     ..))
-  )
+  )%pred
   (at level 0, post at level 90, ra closed binder, rb closed binder, only parsing).
 
 (**
@@ -41,56 +43,60 @@ Notation "'RET' : ^( ra , .. , rb ) post" :=
   * propositions about the hashmap machine state.
   * The pre-hashmap must be a subset of both the post- and crash-hashmaps.
   *)
-Notation "{< e1 .. e2 , 'PERM' : pr 'PRE' : pre 'POST' : post >} 'SECURE' p1" :=
-  (forall T (rx: _ -> prog T), corr2 pr
-   (fun pr' done_ s =>
-    (exists e1, ( .. (exists e2,
-     pre s /\
-     (forall r_ ,
-        corr2 pr (fun pr' done'_ s' =>
-           post s' r_ /\
-           done'_ = done_) (rx r_)) /\
-     permission_secure s p1
-     ) .. ))
-   )
-    pr (Bind p1 rx)) 
+Notation "{< e1 .. e2 , 'PERM' : pr 'PRE' : pre 'POST' : post >} p1" :=
+  (forall T (rx: _ -> prog T), corr2
+   (fun done_ bm =>
+    (exis (fun e1 => .. (exis (fun e2 =>
+     exists F_,
+     F_ * pre *
+     [[ forall r_ ,
+        corr2 pr (fun done'_ bm'  =>
+           post F_ r_ * [[ bm' = bm ]] *
+           [[ done'_ = done_ ]])%pred (rx r_) ]]
+     )) .. ))
+   )%pred
+   (Bind p1 rx)%pred)
   (at level 0, p1 at level 60,
     e1 closed binder, e2 closed binder).
 
 Theorem pimpl_ok2:
-  forall T pr (pre pre': perm -> donecond T -> state -> Prop) (p: prog T),
+  forall T pr  (pre pre': donecond T -> block_mem -> @pred _ _ tagged_block) (p: prog T),
   corr2 pr pre' p ->
-  (forall pr' done s, pre pr' done s  ->  pre' pr' done s) ->
+  (forall done bm, pre done bm =p=>  pre' done bm) ->
   corr2 pr pre p.
 Proof.
   unfold corr2; intros.
   eapply H; eauto.
+  apply H0; auto.
 Qed.
 
 Theorem pimpl_ok2_cont :
-  forall T pr (pre pre': perm -> donecond T -> state -> Prop) A (k : A -> prog T) x y,
+  forall T pr (pre pre': donecond T -> block_mem -> @pred _ _ tagged_block) A (k : A -> prog T) x y,
     corr2 pr pre' (k y) ->
-    (forall pr' done s, pre pr' done s  ->  pre' pr' done s) ->
-    (forall pr' done s, pre pr' done s  -> x = y) ->
+    (forall done bm, pre done bm  =p=>  pre' done bm) ->
+    (forall done bm, pre done bm  =p=> [x = y]) ->
     corr2 pr pre (k x).
 Proof.
   unfold corr2; intros.
   edestruct H1; eauto.
+  eapply H; eauto.
+  apply H0; auto.
 Qed.
 
 Theorem pimpl_pre2:
-  forall T pr pre' (pre: perm -> donecond T -> state -> Prop) (p: prog T),
-    (forall pr' done s, pre pr' done s  ->  corr2 pr (pre' pr' done s) p) ->
-    (forall pr' done s, pre pr' done s  -> pre' pr' done s pr' done s) ->
+  forall T pr pre' (pre: donecond T -> block_mem -> @pred _ _ tagged_block) (p: prog T),
+    (forall done bm, pre done bm  =p=>  [corr2 pr (pre' done bm) p]) ->
+    (forall done bm, pre done bm  =p=> pre' done bm done bm) ->
     corr2 pr pre p.
 Proof.
   unfold corr2; intros.
   eapply H; eauto.
+  apply H0; auto.
 Qed.
 
 Theorem pre_false2:
-  forall T pr (pre: perm -> donecond T -> state -> Prop) (p: prog T),
-    (forall pr' done s, pre pr' done s  ->  False) ->
+  forall T pr (pre: donecond T -> block_mem -> @pred _ _ tagged_block) (p: prog T),
+    (forall done bm, pre done bm  =p=>  [False]) ->
     corr2 pr pre p.
 Proof.
   unfold corr2; intros; exfalso.
@@ -99,8 +105,8 @@ Qed.
 
 Theorem corr2_exists:
   forall T R pr pre (p: prog R),
-    (forall (a:T), corr2 pr (fun pr' done s => pre pr' done s a) p) ->
-    corr2 pr (fun pr' done s => exists a:T, pre pr' done s a) p.
+    (forall (a:T), corr2 pr (fun done bm => pre done bm a) p) ->
+    corr2 pr (fun done bm => exists a:T, pre done bm a)%pred p.
 Proof.
   unfold corr2; intros.
   destruct H0.
@@ -109,9 +115,10 @@ Qed.
 
 Theorem corr2_forall:
     forall T R pr pre (p: prog R),
-      corr2 pr (fun pr' done s => exists a:T, pre pr' done s a) p ->
-  (forall (a:T), corr2 pr (fun pr' done s => pre pr' done s a) p).
+      corr2 pr (fun done bm => exists a:T, pre done bm a)%pred p ->
+  (forall (a:T), corr2 pr (fun done bm => pre done bm a) p).
 Proof.
   unfold corr2; intros.
   eapply H; eauto.
+  exists a; auto.
 Qed.
